ulib/FStar.Reflection.Types.fsti
@@ -19,9 +19,11 @@ include FStar.Range
 include FStar.VConfig
 include FStar.Sealed
 
+assume new type namedv  // named fresh variable
+assume new type bv      // db variable
 assume new type binder
-assume new type bv     // db variable
-assume new type namedv // named fresh variable
+assume new type binding // a named binding with type, e.g. in an environment
+
 assume new type term
 assume new type env
 assume new type fv
