ulib/FStar.Tactics.NamedView.fst
@@ -1,0 +1,135 @@
+(*
+   Copyright 2008-2018 Microsoft Research
+
+   Licensed under the Apache License, Version 2.0 (the "License");
+   you may not use this file except in compliance with the License.
+   You may obtain a copy of the License at
+
+       http://www.apache.org/licenses/LICENSE-2.0
+
+   Unless required by applicable law or agreed to in writing, software
+   distributed under the License is distributed on an "AS IS" BASIS,
+   WITHOUT WARRANTIES OR CONDITIONS OF ANY KIND, either express or implied.
+   See the License for the specific language governing permissions and
+   limitations under the License.
+*)
+module FStar.Tactics.NamedView
+
+open FStar.Reflection
+open FStar.Tactics.Effect
+open FStar.Tactics.Builtins
+
+module RD = FStar.Reflection.Data
+
+(** FIXME: needs named version. *)
+noeq
+type pattern =
+ // A built-in constant
+ | Pat_Constant {
+     c : vconst
+   }
+
+ // A fully applied constructor, each boolean marks whether the
+ // argument was an explicitly-provided implicit argument
+ | Pat_Cons {
+     head    : fv;
+     univs   : option universes;
+     subpats : list (pattern * bool)
+   }
+
+ // A pattern-bound *named* variable. 
+ | Pat_Var {
+     v    : namedv;
+     sort : sealed typ;
+   }
+
+ // Dot pattern: resolved by other elements in the pattern and type
+ | Pat_Dot_Term {
+     t : option term;
+   }
+
+noeq
+type named_binder = {
+  ppname : ppname_t;
+  uniq   : nat;
+  sort   : typ;
+  qual   : aqualv;
+  attrs  : list term;
+}
+
+type simple_named_binder = b:named_binder{Q_Explicit? b.qual /\ Nil? b.attrs}
+
+noeq
+type named_term_view =
+  | Tv_Var    : v:namedv -> named_term_view
+  | Tv_BVar   : v:bv -> named_term_view
+  | Tv_FVar   : v:fv -> named_term_view
+  | Tv_UInst  : v:fv -> us:universes -> named_term_view
+  | Tv_App    : hd:term -> a:argv -> named_term_view
+  | Tv_Abs    : bv:named_binder -> body:term -> named_term_view
+  | Tv_Arrow  : bv:named_binder -> c:comp -> named_term_view
+  | Tv_Type   : universe -> named_term_view
+  | Tv_Refine : b:simple_named_binder -> ref:term -> named_term_view
+  | Tv_Const  : vconst -> named_term_view
+  | Tv_Uvar   : nat -> ctx_uvar_and_subst -> named_term_view
+  | Tv_Let    : recf:bool -> attrs:(list term) -> b:simple_named_binder -> def:term -> body:term -> named_term_view
+  | Tv_Match  : scrutinee:term -> ret:option match_returns_ascription -> brs:(list branch) -> named_term_view
+  | Tv_AscribedT : e:term -> t:term -> tac:option term -> use_eq:bool -> named_term_view
+  | Tv_AscribedC : e:term -> c:comp -> tac:option term -> use_eq:bool -> named_term_view
+  | Tv_Unknown  : named_term_view // An underscore: _
+  | Tv_Unsupp : named_term_view // failed to inspect, not supported
+
+let term_view = named_term_view
+
+let binding_to_named_binder (bnd : binding) (b : binder) : named_binder =
+  let bndv = inspect_binding bnd in
+  {
+      ppname = bndv.ppname;
+      uniq   = bndv.uniq;
+      sort   = bndv.sort;
+      qual   = (inspect_binder b).qual;
+      attrs  = (inspect_binder b).attrs;
+  }
+
+let inspect (t:term) : Tac named_term_view =
+  let tv = inspect_ln t in
+  match tv with
+  (* Nothing interesting *)
+  | RD.Tv_Var v -> Tv_Var v
+  | RD.Tv_BVar v -> Tv_BVar v
+  | RD.Tv_FVar v -> Tv_FVar v
+  | RD.Tv_UInst v us -> Tv_UInst v us
+  | RD.Tv_App hd a -> Tv_App hd a
+  | RD.Tv_Type u -> Tv_Type u
+  | RD.Tv_Const c -> Tv_Const c
+  | RD.Tv_Uvar n ctx_uvar_and_subst -> Tv_Uvar n ctx_uvar_and_subst
+  | RD.Tv_AscribedT e t tac use_eq -> Tv_AscribedT e t tac use_eq
+  | RD.Tv_AscribedC e c tac use_eq -> Tv_AscribedC e c tac use_eq
+  | RD.Tv_Unknown -> Tv_Unknown
+  | RD.Tv_Unsupp -> Tv_Unsupp
+
+  (* Below are the nodes that actually involve a binder.
+  Open them and convert to named binders. *)
+
+  | RD.Tv_Abs b body ->
+    let bnd, body = open_term b body in
+    let nb = binding_to_named_binder bnd b in
+    Tv_Abs nb body
+
+  | RD.Tv_Arrow b c ->
+    let bnd, body = open_comp b c in
+    let nb = binding_to_named_binder bnd b in
+    Tv_Arrow nb c
+
+  | RD.Tv_Refine b ref ->
+    let bnd, ref = open_term b ref in
+    let nb = binding_to_named_binder bnd b in
+    Tv_Refine nb ref
+
+  | RD.Tv_Let recf attrs b def body ->
+    let bnd, body = open_term b body in
+    let nb = binding_to_named_binder bnd b in
+    Tv_Let recf attrs nb def body
+
+  (* FIXME *)
+  | RD.Tv_Match scrutinee ret brs -> Tv_Match scrutinee ret brs
