ulib/FStar.Tactics.fst
@@ -33,3 +33,4 @@ include FStar.Tactics.Util
 include FStar.Tactics.SyntaxHelpers
 include FStar.Tactics.Print
 include FStar.Tactics.Visit
+include FStar.Tactics.NamedView
